haskell/Optics/Optics/Singleton.hs
@@ -1,0 +1,21 @@
+{-# LANGUAGE PolyKinds              #-}
+{-# LANGUAGE TypeFamilies           #-}
+{-# LANGUAGE KindSignatures         #-}
+
+module  Optics.Singleton
+    (   Sing 
+    ,   SingE   (..)  
+    )   where
+
+data family Sing (a :: k) 
+
+
+instance Eq (Sing a) where
+    (==) _ _ = True
+
+
+class SingE (a :: k) where
+    type Demote a
+    fromSing :: Sing a -> Demote a
+
+
