coq/ref/CIC.v
@@ -1,3 +1,7 @@
+Require Import List.
+Import ListNotations.
+
+(* Abstract syntax for 'calculus of inductive constructions'.                   *)
 Inductive Exp : Type :=
 | EProp : Exp                               (* sort 'Prop'                      *)
 | ESet  : Exp                               (* sort 'Set'                       *)
@@ -10,13 +14,30 @@ Inductive Exp : Type :=
 | ELet  : nat -> Exp -> Exp -> Exp -> Exp   (* let x:=(t:T) in U                *)
 .
 
+(* Whether a term is a 'sort' or not. Needed to defined typing rules.           *)
+Inductive isSort : Exp -> Prop :=
+| SortProp : isSort EProp
+| SortSet  : isSort ESet
+| SortType : forall (n:nat), isSort (EType n)
+.
+
+(* Type for 'local declaration'                                                 *)
 Inductive LocalDecl : Type :=
 | LAssume : nat -> Exp -> LocalDecl         (* x:T , T is a type                *)
 | LDefine : nat -> Exp -> Exp -> LocalDecl  (* x := (t:T)                       *)
 .
 
+Definition declVar (decl:LocalDecl) : nat :=
+    match decl with
+    | LAssume n _   => n
+    | LDefine n _ _ => n
+    end.
+
 (* variable involved must be distinct                                           *)
 Definition LocalContext : Type := list LocalDecl. 
+
+Definition inLocCtx (n:nat) (ctx:LocalContext) : Prop := 
+    In n (map declVar ctx).
 
 Inductive GlobalDecl : Type :=
 | GAssume : nat -> Exp -> GlobalDecl        (* c:T, T is a type                 *)
@@ -34,5 +55,21 @@ Definition GlobalEnv : Type := list GlobalDecl.
 
 (* Definition: t is well-typed in E, iff there exists a local context C         *)
 (* and a term T such that E[C] |- t:T can be derived from typing rules          *)
+
+Inductive Entails : GlobalEnv -> LocalContext -> Exp -> Exp -> Prop :=
+
+
+with WF : GlobalEnv -> LocalContext -> Prop :=  
+| WEmpty: WF [] []
+| WLocalAssume: forall env ctx T s n, 
+    Entails env ctx T s -> 
+    isSort s            -> 
+    ~ inLocCtx n ctx    -> 
+    WF env ((LAssume n T) :: ctx) 
+| WLocalDef: forall env ctx t T n,
+    Entails env ctx t T ->
+    ~ inLocCtx n ctx    ->
+    WF env ((LDefine n t T) :: ctx)
+.
 
 
