coq/set/Core/Environment.v
@@ -1,0 +1,29 @@
+Require Import Core.Nat.
+Require Import Core.Set.
+
+Definition Env : Type := nat -> set.
+
+(* Safe environment allowing variables to be unbound leading to error checking. *)
+Definition Env' : Type := nat -> option set.
+
+Definition eDef  : Env  := (fun _ => Nil).
+Definition eDef' : Env' := (fun _ => None).
+
+(* Tweak environment e to that e n = x                                          *)
+Definition bind (e:Env) (n:nat) (x:set) : Env :=
+    fun (m:nat) =>
+        match eq_nat_dec n m with
+        | left _    => x        (* variable 'n' is bound to set 'x'             *)
+        | right _   => e m
+        end.
+
+(* Tweak environment e to that e n = x                                          *)
+Definition bind' (e:Env') (n:nat) (x:set) : Env' :=
+    fun (m:nat) =>
+        match eq_nat_dec n m with
+        | left _    => Some x   (* variable 'n' is bound to set 'x'             *)
+        | right _   => e m
+        end.
+
+(* Environment with single binding n := x, variable 'n' is bound to set 'x'.    *)
+Definition env (n:nat) (x:set) : Env := bind eDef n x.
